src/Mem.v
@@ -1,6 +1,5 @@
 Require Import Arith.
 Require Import Word.
-Require Import Bytes.
 Require Import Eqdep_dec.
 Require Import FunctionalExtensionality.
 
@@ -87,56 +86,8 @@ End Valulen.
 
 Definition addrlen := 64.
 Notation "'valulen'" := (Valulen.valulen).
-Notation "'valubytes'" := (Valulen.valubytes).
 Notation "'valulen_is'" := (Valulen.valulen_is).
-Notation "'valubytes_is'" := (Valulen.valubytes_is).
-
-Notation "'addr'" := nat.
-Notation "'waddr'" := (word addrlen).
 Notation "'valu'" := (word valulen).
-
-Definition addr_eq_dec := Nat.eq_dec.
-Definition waddr_eq_dec := @weq addrlen.
-
-Definition valu2bytes (v : valu) : bytes valubytes.
-  refine (@word2bytes valulen valubytes _ v).
-  rewrite valulen_is. rewrite valubytes_is. reflexivity.
-Defined.
-
-Definition bytes2valu (v : bytes valubytes) : valu.
-  rewrite valulen_is.
-  unfold bytes in *.
-  rewrite valubytes_is in *.
-  exact v.
-Defined.
-
-Theorem valu2bytes2valu : forall v, valu2bytes (bytes2valu v) = v.
-Proof.
-  unfold valu2bytes, bytes2valu, eq_rec_r, eq_rec.
-  intros.
-  rewrite eq_rect_word_mult.
-  rewrite eq_rect_nat_double.
-  generalize dependent v.
-  rewrite valubytes_is.
-  rewrite valulen_is.
-  intros.
-  rewrite <- (eq_rect_eq_dec eq_nat_dec).
-  reflexivity.
-Qed.
-
-Theorem bytes2valu2bytes : forall v, bytes2valu (valu2bytes v) = v.
-Proof.
-  unfold valu2bytes, bytes2valu, eq_rec_r, eq_rec.
-  intros.
-  rewrite eq_rect_word_mult.
-  rewrite eq_rect_nat_double.
-  generalize dependent v.
-  rewrite valubytes_is.
-  rewrite valulen_is.
-  intros.
-  rewrite <- (eq_rect_eq_dec eq_nat_dec).
-  reflexivity.
-Qed.
 
 Theorem valulen_wordToNat_natToWord : # (natToWord addrlen valulen) = valulen.
 Proof.
@@ -155,5 +106,12 @@ Proof.
 Qed.
 
 
-Definition wringaddr := wring addrlen.
-Add Ring wringaddr : wringaddr (decidable (weqb_sound addrlen), constants [wcst]).
+Notation "'addr'" := nat.
+Notation "'waddr'" := (word addrlen).
+
+Definition addr_eq_dec := Nat.eq_dec.
+Definition waddr_eq_dec := @weq addrlen.
+
+Definition waddrring := wring addrlen.
+Add Ring waddrring : waddrring (decidable (weqb_sound addrlen), constants [wcst]).
+
